VHDL_Hoare.thy
@@ -1,0 +1,650 @@
+(*
+ * Copyright 2018, NTU
+ *
+ * This software may be distributed and modified according to the terms of
+ * the BSD 2-Clause license. Note that NO WARRANTY is provided.
+ * See "LICENSE_BSD2.txt" for details.
+ *
+ *  Author: Albert Rizaldi, NTU Singapore
+ *)
+
+theory VHDL_Hoare
+  imports Femto_VHDL
+begin
+
+subsection \<open>Hoare Logic for @{typ "'signal seq_stmt"}\<close>
+
+type_synonym 'signal worldline = "'signal \<Rightarrow> nat \<Rightarrow> val"
+
+definition worldline_upd :: "'signal worldline \<Rightarrow> 'signal \<Rightarrow> nat \<Rightarrow> val \<Rightarrow> 'signal worldline" ("_[_, _:= _]") where
+  "worldline_upd w s t v = (\<lambda>s' t'. if s' \<noteq> s \<or> t' < t then w s' t' else v)"
+
+definition worldline_inert_upd :: "'signal worldline \<Rightarrow> 'signal \<Rightarrow> nat \<Rightarrow> nat \<Rightarrow> val \<Rightarrow> 'signal worldline" ("_[_, _, _ := _]") where
+  "worldline_inert_upd w s t t0 v = (\<lambda>s' t'. if s' \<noteq> s \<or> t' < t0 then w s' t' else if t' < t then w s' t0 else v)"
+
+type_synonym 'signal assn = "'signal worldline \<Rightarrow> bool"
+
+definition state_of_world :: "'signal worldline \<Rightarrow> nat \<Rightarrow> 'signal state" where
+  "state_of_world w t = (\<lambda>s. w s t)"
+
+definition event_of_world :: "'signal worldline \<Rightarrow> nat \<Rightarrow> 'signal event" where
+  "event_of_world w t = (if t = 0 then {s :: 'signal. w s 0 \<noteq> False} else {s :: 'signal. w s t \<noteq> w s (t - 1)})"
+
+definition beh_of_world_raw :: "'signal worldline \<Rightarrow> nat \<Rightarrow> nat \<Rightarrow> 'signal \<rightharpoonup> val" where
+  "beh_of_world_raw w t = (\<lambda>t'. if t' < t then (\<lambda>s. Some (w s t')) else Map.empty)"
+
+lift_definition beh_of_world :: "'signal worldline \<Rightarrow> nat \<Rightarrow> 'signal transaction" is beh_of_world_raw
+  unfolding beh_of_world_raw_def zero_map by auto
+
+lemma [simp]:
+  "beh_of_world w 0 = 0"
+  by (transfer', auto simp add:  beh_of_world_raw_def zero_option_def zero_fun_def)
+
+definition beval_world :: "'signal worldline \<Rightarrow> nat \<Rightarrow> 'signal bexp \<Rightarrow> val" where
+  "beval_world w t exp = beval t (state_of_world w t) (event_of_world w t) (beh_of_world w t) exp"
+
+definition trans_of_world_raw :: "'signal worldline \<Rightarrow> nat \<Rightarrow> nat \<Rightarrow> 'signal \<rightharpoonup> val" where
+  "trans_of_world_raw w t = (\<lambda>t'. if t \<le> t' then undefined else Map.empty)"
+
+inductive
+  seq_hoare :: "nat \<Rightarrow> 'signal assn \<Rightarrow> 'signal seq_stmt \<Rightarrow> 'signal assn \<Rightarrow> bool" ("\<turnstile>\<^sub>_ ({(1_)}/ (_)/ {(1_)})" 50)
+  where
+Null: "\<turnstile>\<^sub>t {P} Bnull {P}" |
+
+Assign: "\<turnstile>\<^sub>t {\<lambda>w. P(w[sig, t + dly := beval_world w t exp])} Bassign_trans sig exp dly {P}" |
+
+AssignI: "\<turnstile>\<^sub>t {\<lambda>w. P(w[sig, t + dly, t := beval_world w t exp])} Bassign_inert sig exp dly {P}" |
+
+Comp: "\<lbrakk> \<turnstile>\<^sub>t {P} s1 {Q}; \<turnstile>\<^sub>t {Q} s2 {R}\<rbrakk> \<Longrightarrow> \<turnstile>\<^sub>t {P} Bcomp s1 s2 {R}" |
+
+If: "\<lbrakk>\<turnstile>\<^sub>t {\<lambda>w. P w \<and> beval_world w t g} s1 {Q}; \<turnstile>\<^sub>t {\<lambda>w. P w \<and> \<not> beval_world w t  g} s2 {Q}\<rbrakk>
+        \<Longrightarrow>  \<turnstile>\<^sub>t {P} Bguarded g s1 s2 {Q}" |
+
+Conseq: "\<lbrakk>\<forall>w. P' w \<longrightarrow> P w; \<turnstile>\<^sub>t {P} s {Q}; \<forall>w. Q w \<longrightarrow> Q' w\<rbrakk> \<Longrightarrow> \<turnstile>\<^sub>t {P'} s {Q'}"
+
+inductive_cases seq_hoare_ic: "\<turnstile>\<^sub>t {P} s {Q}"
+
+lemma BnullE:
+  assumes "\<turnstile>\<^sub>t {P} s {Q}"
+  assumes "s = Bnull"
+  shows "\<forall>w. P w \<longrightarrow> Q w"
+  using assms
+  by (induction rule:seq_hoare.induct, auto)
+
+lemma BnullE':
+  "\<turnstile>\<^sub>t {P} Bnull {Q} \<Longrightarrow> \<forall>w. P w \<longrightarrow> Q w"
+  using BnullE by blast
+
+lemma BassignE:
+  assumes "\<turnstile>\<^sub>t {P} s {Q}"
+  assumes "s = Bassign_trans sig exp dly"
+  shows "\<forall>w. P w \<longrightarrow> Q(w[sig, t + dly := beval_world w t exp])"
+  using assms
+  by (induction rule: seq_hoare.induct, auto)
+
+lemma Bassign_inertE:
+  assumes "\<turnstile>\<^sub>t {P} s {Q}"
+  assumes "s = Bassign_inert sig exp dly"
+  shows "\<forall>w. P w \<longrightarrow> Q(w[sig, t + dly, t := beval_world w t exp])"
+  using assms
+  by (induction rule: seq_hoare.induct, auto)
+
+lemma BcompE:
+  assumes "\<turnstile>\<^sub>t {P} s {R}"
+  assumes "s = Bcomp s1 s2"
+  shows "\<exists>Q. \<turnstile>\<^sub>t {P} s1 {Q} \<and> \<turnstile>\<^sub>t {Q} s2 {R}"
+  using assms Conseq
+  by (induction rule:seq_hoare.induct, auto) (blast)
+
+lemmas [simp] = seq_hoare.Null seq_hoare.Assign seq_hoare.Comp seq_hoare.If
+lemmas [intro!] = seq_hoare.Null seq_hoare.Assign seq_hoare.Comp seq_hoare.If
+
+lemma strengthen_pre:
+  assumes "\<forall>w. P' w \<longrightarrow> P w" and "\<turnstile>\<^sub>t {P} s {Q}"
+  shows "\<turnstile>\<^sub>t {P'} s {Q}"
+  using assms by (blast intro: Conseq)
+
+lemma weaken_post:
+  assumes "\<forall>w. Q w \<longrightarrow> Q' w" and "\<turnstile>\<^sub>t {P} s {Q}"
+  shows "\<turnstile>\<^sub>t {P} s {Q'}"
+  using assms by (blast intro: Conseq)
+
+lemma Assign':
+  assumes "\<forall>w. P w \<longrightarrow> Q (worldline_upd w sig (t + dly) (beval_world w t exp))"
+  shows "\<turnstile>\<^sub>t {P} Bassign_trans sig exp dly {Q}"
+  using assms by (simp add: strengthen_pre)
+
+subsection \<open>Validity of Hoare proof rules\<close>
+
+definition worldline :: "nat \<Rightarrow> 'signal state \<Rightarrow> 'signal transaction \<Rightarrow> 'signal transaction \<Rightarrow> 'signal worldline" where
+  "worldline t \<sigma> \<theta> \<tau> = (\<lambda>s' t'. if t' < t then signal_of2 False \<theta> s' t' else signal_of2 (\<sigma> s') \<tau> s' t')"
+
+definition
+seq_hoare_valid :: "nat \<Rightarrow> 'signal assn \<Rightarrow> 'signal seq_stmt \<Rightarrow> 'signal assn \<Rightarrow> bool" ("\<Turnstile>\<^sub>_ {(1_)}/ (_)/ {(1_)}" 50)
+  where "\<Turnstile>\<^sub>t {P} s {Q} \<longleftrightarrow>  (\<forall>\<sigma> \<tau> \<gamma> \<theta> \<tau>' w w'.  context_invariant t \<sigma> \<gamma> \<theta> \<tau>
+                                            \<and>  w = worldline t \<sigma> \<theta> \<tau>
+                                            \<and>  P w
+                                            \<and> (t, \<sigma>, \<gamma>, \<theta> \<turnstile> <s, \<tau>> \<longrightarrow>\<^sub>s \<tau>')
+                                            \<and>  w' = worldline t \<sigma> \<theta> \<tau>' \<longrightarrow> Q w')"
+
+lemma Bcomp_hoare_valid:
+  assumes "\<Turnstile>\<^sub>t {P} s1 {Q}" and "\<Turnstile>\<^sub>t {Q} s2 {R}"
+  assumes "nonneg_delay (Bcomp s1 s2)"
+  shows "\<Turnstile>\<^sub>t {P} Bcomp s1 s2 {R}"
+  unfolding seq_hoare_valid_def
+proof (rule)+
+  fix \<sigma> :: "'a state"
+  fix \<tau> \<theta> \<tau>' :: "'a transaction"
+  fix \<gamma> :: "'a event"
+  fix w w' :: "'a worldline"
+  assume "context_invariant t \<sigma> \<gamma> \<theta> \<tau> \<and> w = worldline t \<sigma> \<theta> \<tau> \<and> P w \<and>
+          t , \<sigma> , \<gamma> , \<theta> \<turnstile> <Bcomp s1 s2 , \<tau>> \<longrightarrow>\<^sub>s \<tau>' \<and> w' = worldline t \<sigma> \<theta> \<tau>'"
+  hence "context_invariant t \<sigma> \<gamma> \<theta> \<tau>" and "w = worldline t \<sigma> \<theta> \<tau>" and "P w"
+    and "t , \<sigma> , \<gamma> , \<theta> \<turnstile> <Bcomp s1 s2 , \<tau>> \<longrightarrow>\<^sub>s \<tau>' " and 2: "w' = worldline t \<sigma> \<theta> \<tau>'"
+    by auto
+  then obtain \<tau>'' where 0: "t, \<sigma>, \<gamma>, \<theta> \<turnstile> <s1, \<tau>> \<longrightarrow>\<^sub>s \<tau>''" and 1: "t, \<sigma>, \<gamma>, \<theta> \<turnstile> <s2, \<tau>''> \<longrightarrow>\<^sub>s \<tau>'"
+    by auto
+  define w'' where "w'' = worldline t \<sigma> \<theta> \<tau>''"
+  hence "Q w''"
+    using `\<Turnstile>\<^sub>t {P} s1 {Q}` unfolding seq_hoare_valid_def
+    using \<open>P w\<close> \<open>context_invariant t \<sigma> \<gamma> \<theta> \<tau>\<close> \<open>t , \<sigma> , \<gamma> , \<theta> \<turnstile> <s1 , \<tau>> \<longrightarrow>\<^sub>s \<tau>''\<close> \<open>w = worldline t \<sigma> \<theta> \<tau>\<close>
+    by blast
+  have "context_invariant t \<sigma> \<gamma> \<theta> \<tau>''"
+    using b_seq_exec_preserves_context_invariant[OF `context_invariant t \<sigma> \<gamma> \<theta> \<tau>` 0] assms(3)
+    by auto
+  thus "R w'"
+    using `\<Turnstile>\<^sub>t {Q} s2 {R}` `w'' = worldline t \<sigma> \<theta> \<tau>''` `Q w''` 1 2 unfolding seq_hoare_valid_def
+    by auto
+qed
+
+(*      Relationship between w, \<tau>, \<tau>', and w'  in seq_hoare_valid
+ *
+ *         P w             \<longrightarrow>               Q w
+ *          \<up>                                 \<up>
+ * w = worldline t \<sigma> \<theta> \<tau>          w' = worldline t \<sigma> \<theta> \<tau>'
+ *          \<up>                                 \<up>
+ *          \<tau>              \<longrightarrow>\<^sub>c               \<tau>'
+ *
+ *)
+
+lemma Bnull_sound:
+  "\<turnstile>\<^sub>t {P} Bnull {Q} \<Longrightarrow> \<Turnstile>\<^sub>t {P} Bnull {Q}"
+  by (auto dest!: BnullE' simp add: seq_hoare_valid_def)
+
+lemma state_of_world:
+  assumes "w = worldline t \<sigma> \<theta> \<tau>"
+  assumes "\<And>n. n < t \<Longrightarrow> lookup \<tau> n = 0"
+  assumes "\<And>s. s \<in> dom (lookup \<tau> t) \<Longrightarrow> \<sigma> s = the (lookup \<tau> t s)"
+  shows "state_of_world w t = \<sigma>"
+proof
+  fix x
+  have "signal_of2 (\<sigma> x) \<tau> x t = \<sigma> x"
+  proof (cases "lookup (to_transaction2 \<tau> x) t = 0")
+    case True
+    hence "\<forall>k \<in> dom (lookup (to_transaction2 \<tau> x)). t \<le> k"
+      using assms(2) apply transfer' unfolding to_trans_raw2_def
+      by (metis (full_types) domIff not_less zero_map)
+    moreover have "t \<notin> dom (lookup (to_transaction2 \<tau> x))"
+      using True  by (simp add: domIff zero_option_def)
+    ultimately have "\<forall>k \<in> dom (lookup (to_transaction2 \<tau> x)). t < k"
+      using nat_less_le by auto
+    hence "inf_time (to_transaction2 \<tau>) x t = None"
+      by (auto intro:inf_time_noneI)
+    thus "signal_of2 (\<sigma> x) \<tau> x t = \<sigma> x"
+      unfolding to_signal2_def comp_def by auto
+  next
+    case False
+    hence "x \<in> dom (get_trans \<tau> t)"
+      by (transfer', simp add: domIff zero_option_def to_trans_raw2_def)
+    hence "\<sigma> x = the (lookup \<tau> t x)"
+      using assms(3) by auto
+    hence "lookup \<tau> t x = (Some \<circ> \<sigma>) x"
+      using \<open>x \<in> dom (get_trans \<tau> t)\<close> domIff by auto
+    thus "signal_of2 (\<sigma> x) \<tau> x t = \<sigma> x"
+      using lookup_some_signal_of2' by fastforce
+  qed
+  thus "state_of_world w t x = \<sigma> x"
+    unfolding state_of_world_def assms worldline_def by auto
+qed
+
+lemma beval_beh_of_world:
+  assumes "w = worldline t \<sigma> \<theta> \<tau>"
+  assumes "\<And>n. t \<le> n \<Longrightarrow> lookup \<theta> n = 0"
+  shows "beval t \<sigma> \<gamma> (beh_of_world w t) exp = beval t \<sigma> \<gamma> \<theta> exp"
+  using assms
+proof (induction exp)
+  case (Bsig_delayed sig n)
+  have "t , \<sigma> , \<gamma> , beh_of_world w t \<turnstile> Bsig_delayed sig n \<longrightarrow>\<^sub>b signal_of2 False (beh_of_world w t) sig (t - n)"
+    by auto
+  have *: "beval t \<sigma> \<gamma> \<theta> (Bsig_delayed sig n) = signal_of2 False \<theta> sig (t - n)"
+    by auto
+  have "0 < n \<and> 0 < t \<or> (t \<noteq> 0 \<and> n = 0) \<or> t = 0"
+    by auto
+  moreover
+  { assume "0 < n \<and> 0 < t"
+    hence "get_trans (beh_of_world w t) (t - n) = Some \<circ> (\<lambda>s. w s (t - n))"
+      apply transfer' unfolding beh_of_world_raw_def comp_def by auto
+    hence "signal_of2 False (beh_of_world w t) sig (t - n) = w sig (t - n)"
+      by (auto dest!: lookup_some_signal_of2)
+    also have "... = signal_of2 False \<theta> sig (t - n)"
+      using `0 < n \<and> 0 < t` unfolding assms worldline_def by auto
+    also have "... = beval t \<sigma> \<gamma> \<theta> (Bsig_delayed sig n)"
+      using * by auto
+    finally have "signal_of2 False (beh_of_world w t) sig (t - n) = beval t \<sigma> \<gamma> \<theta> (Bsig_delayed sig n)"
+      by auto
+    hence ?case by auto }
+
+  moreover
+  { assume "t \<noteq> 0 \<and> n = 0 \<or> t = 0"
+    moreover
+    { assume "t = 0"
+      hence "t - n = 0" by auto
+      have "beh_of_world w t = 0" unfolding `t = 0` by auto
+      hence "signal_of2 False (beh_of_world w t) sig (t - n) = signal_of2 False 0 sig 0"
+        unfolding `t - n = 0` by auto
+      also have "... = False"
+        using signal_of2_empty[of "False" "sig" "0"] by auto
+      finally have "signal_of2 False (beh_of_world w t) sig (t - n) = False"
+        by auto
+      have "\<theta> = 0"
+        using assms(2) unfolding `t = 0` by (transfer', auto)
+      hence "beval t \<sigma> \<gamma> \<theta> (Bsig_delayed sig n) = signal_of2 False \<theta> sig 0"
+        using `t - n = 0` by auto
+      also have "... = False"
+        unfolding `\<theta> = 0` using signal_of2_empty[of "False"] by metis
+      finally have "beval t \<sigma> \<gamma> \<theta> (Bsig_delayed sig n) = False"
+        by auto
+      hence ?case
+        using `signal_of2 False (beh_of_world w t) sig (t - n) = False` by auto }
+    moreover
+    { assume "t \<noteq> 0 \<and> n = 0"
+      have "lookup \<theta> t = 0"
+        using assms(2) by auto
+      have "lookup (beh_of_world w t) t = 0"
+        apply transfer' unfolding beh_of_world_raw_def
+        by (metis (full_types) less_not_refl map_add_subsumed1 map_add_subsumed2 map_le_def zero_map)
+      have *: "lookup (beh_of_world w t) (t - 1) = Some o (\<lambda>s. w s (t - 1))"
+        using `t \<noteq> 0 \<and> n = 0` apply transfer' unfolding beh_of_world_raw_def by auto
+      have "signal_of2 False (beh_of_world w t) sig (t - n) = signal_of2 False (beh_of_world w t) sig t"
+        using `t \<noteq> 0 \<and> n = 0` by auto
+      also have "... = signal_of2 False (beh_of_world w t) sig (t - 1)"
+        using signal_of2_less[OF `lookup (beh_of_world w t) t = 0`] by metis
+      also have "... = w sig (t - 1)"
+        using * by(auto dest!: lookup_some_signal_of2)
+      also have "... = signal_of2 False \<theta> sig (t - 1)"
+        using `t \<noteq> 0 \<and> n = 0` unfolding assms(1) worldline_def by auto
+      also have "... = signal_of2 False \<theta> sig t"
+        using signal_of2_less[OF `lookup \<theta> t = 0`] by metis
+      also have "... = signal_of2 False \<theta> sig (t - n)"
+        using `t \<noteq> 0 \<and> n = 0` by auto
+      finally have "signal_of2 False (beh_of_world w t) sig (t - n) = signal_of2 False \<theta> sig (t - n)"
+        by auto
+      hence ?case
+        by auto }
+    ultimately have ?case by auto }
+  ultimately show ?case by auto
+qed (auto)
+
+text \<open>Note that the definition of @{term "\<gamma>"} below will only be preserved by VHDL code which does
+not contain a zero time signal assignment. That is, in every assignment statement, be it of transport
+or inertial type, must have nonzero delay. Check @{thm "context_invariant"} and note the assumption
+@{term "t < next_time t \<tau>'"}.\<close>
+
+lemma beval_beval_world:
+  assumes "w = worldline t \<sigma> \<theta> \<tau>"
+  assumes "\<And>n. n < t \<Longrightarrow> lookup \<tau> n = 0"
+  assumes gam: "\<gamma> = {s. \<sigma> s \<noteq> signal_of2 False \<theta> s (t - 1)}"
+  assumes "\<And>s. s \<in> dom (lookup \<tau> t) \<Longrightarrow> \<sigma> s = the (lookup \<tau> t s)"
+  assumes beh: "\<And>n. t \<le> n \<Longrightarrow> lookup \<theta> n = 0"
+  shows "beval t \<sigma> \<gamma> \<theta> exp = beval_world w t exp"
+proof -
+  have "state_of_world w t = \<sigma>"
+    using state_of_world[OF assms(1) assms(2) assms(4)] by auto
+  moreover have "event_of_world w t = \<gamma>"
+  proof (cases "0 < t")
+    case True
+    fix s
+    have "w s t = \<sigma> s"
+      using `state_of_world w t = \<sigma>` unfolding state_of_world_def by auto
+    moreover have "w s (t - 1) = signal_of2 False \<theta> s (t - 1)"
+      unfolding assms(1) worldline_def using True by auto
+    ultimately show ?thesis
+      unfolding event_of_world_def assms(3)
+      by (smt Collect_cong \<open>state_of_world w t = \<sigma>\<close> assms(1) True diff_less less_numeral_extra(3)
+          state_of_world_def worldline_def zero_less_one)
+  next
+    case False
+    hence "t = 0" by auto
+    hence ev: "event_of_world w t = {s. w s 0 \<noteq> False}"
+      unfolding event_of_world_def by auto
+    have \<gamma>_def': "\<gamma> = {s. \<sigma> s \<noteq> signal_of2 False \<theta> s 0}"
+      using `t = 0` gam by auto
+    have "\<theta> = 0"
+      using beh unfolding `t = 0` by (simp add: poly_mapping_eqI)
+    hence "\<And>s. signal_of2 False \<theta> s 0 = False"
+      using signal_of2_empty by metis
+    hence "\<gamma> = {s. \<sigma> s \<noteq> False}"
+      using \<gamma>_def' by auto
+    moreover have "\<And>s.  w s 0 = \<sigma> s"
+      using `state_of_world w t = \<sigma>` `t = 0` unfolding state_of_world_def by auto
+    ultimately  have "\<gamma> = {s. w s 0 \<noteq> False}"
+      by auto
+    thus ?thesis  using ev by auto
+  qed
+  ultimately have " beval t (state_of_world w t) (event_of_world w t) (beh_of_world w t) exp =
+                    beval t \<sigma> \<gamma> (beh_of_world w t) exp" by auto
+  also have "... = beval t \<sigma> \<gamma> \<theta> exp"
+    using beval_beh_of_world[OF assms(1) beh] by auto
+  finally show ?thesis
+    unfolding beval_world_def by auto
+qed
+
+lemma Bguarded_hoare_valid:
+  assumes "\<Turnstile>\<^sub>t {\<lambda>a. P a \<and> beval_world a t g} s1 {Q}" and "\<Turnstile>\<^sub>t {\<lambda>a. P a \<and> \<not> beval_world a t g} s2 {Q}"
+  shows "\<Turnstile>\<^sub>t {P} Bguarded g s1 s2 {Q}"
+  unfolding seq_hoare_valid_def
+proof (rule)+
+  fix \<sigma> :: "'a state"
+  fix \<tau> \<theta> \<tau>' :: "'a transaction"
+  fix \<gamma> :: "'a event"
+  fix w w' :: "'a worldline"
+  assume "context_invariant t \<sigma> \<gamma> \<theta> \<tau> \<and> w = worldline t \<sigma> \<theta> \<tau> \<and> P w \<and>
+          t , \<sigma> , \<gamma> , \<theta> \<turnstile> <Bguarded g s1 s2 , \<tau>> \<longrightarrow>\<^sub>s \<tau>' \<and> w' = worldline t \<sigma> \<theta> \<tau>'"
+  hence s: "t , \<sigma> , \<gamma> , \<theta> \<turnstile> <Bguarded g s1 s2 , \<tau>> \<longrightarrow>\<^sub>s \<tau>'" and w: "w = worldline t \<sigma> \<theta> \<tau>"
+    and c: "context_invariant t \<sigma> \<gamma> \<theta> \<tau>" and p: "P w" and w': "w' = worldline t \<sigma> \<theta> \<tau>'"
+    by auto
+  have "beval t \<sigma> \<gamma> \<theta> g \<or> \<not> beval t \<sigma> \<gamma> \<theta> g"
+    by auto
+  moreover
+  { assume "beval t \<sigma> \<gamma> \<theta> g "
+    hence \<tau>'_def: "t , \<sigma> , \<gamma> , \<theta> \<turnstile> <s1 , \<tau>> \<longrightarrow>\<^sub>s \<tau>'"
+      using s by auto
+    have "beval_world w t g"
+      using `beval t \<sigma> \<gamma> \<theta> g` beval_beval_world[OF w _ _ _ _] c unfolding context_invariant_def
+      by auto
+    with `P w` have " Q w'"
+      using assms(1) c w \<tau>'_def w' unfolding seq_hoare_valid_def by auto }
+  moreover
+  { assume "\<not> beval t \<sigma> \<gamma> \<theta> g"
+    hence \<tau>'_def: "t, \<sigma>, \<gamma>, \<theta> \<turnstile> <s2, \<tau>> \<longrightarrow>\<^sub>s \<tau>'"
+      using s by auto
+    have "\<not> beval_world w t g"
+      using `\<not> beval t \<sigma> \<gamma> \<theta> g` beval_beval_world[OF w _ _ _ _] c unfolding context_invariant_def
+      by auto
+    with `P w` have "Q w'"
+      using assms(2) c w \<tau>'_def w' unfolding seq_hoare_valid_def by auto }
+  ultimately show "Q w'" by auto
+qed
+
+lemma Bassign_trans_sound:
+  "\<turnstile>\<^sub>t {P} Bassign_trans sig exp dly {Q} \<Longrightarrow> \<Turnstile>\<^sub>t {P} Bassign_trans sig exp dly {Q}"
+proof -
+  assume "\<turnstile>\<^sub>t {P} Bassign_trans sig exp dly {Q}"
+  hence imp: "\<forall>w. P w \<longrightarrow> Q(w[sig, t + dly := beval_world w t exp])"
+    by (auto dest!: BassignE)
+  { fix \<sigma> :: "'a state"
+    fix \<tau> \<tau>' \<theta> :: "'a transaction"
+    fix w w' :: "'a worldline"
+    fix \<gamma>
+    assume "context_invariant t \<sigma> \<gamma> \<theta> \<tau>"
+    assume "w = worldline t \<sigma> \<theta> \<tau>"
+    assume "P w"
+    assume "t, \<sigma>, \<gamma>, \<theta> \<turnstile> <Bassign_trans sig exp dly, \<tau>> \<longrightarrow>\<^sub>s \<tau>'"
+    hence "\<tau>' = trans_post sig (beval t \<sigma> \<gamma> \<theta> exp) \<tau> (t + dly)"
+      by auto
+    moreover have "beval t \<sigma> \<gamma> \<theta> exp = beval_world w t exp"
+      using `w = worldline t \<sigma> \<theta> \<tau>`  `context_invariant t \<sigma> \<gamma> \<theta> \<tau>`
+      unfolding context_invariant_def by (simp add: beval_beval_world)
+    ultimately have \<tau>'_def: "\<tau>' = trans_post sig (beval_world w t exp) \<tau> (t + dly)"
+      by auto
+    have "worldline t \<sigma> \<theta> \<tau>' = w[sig, t + dly := beval_world w t exp]"
+    proof (rule ext, rule ext)
+      fix s' t'
+      have "t' < t \<or> t' \<ge> t" by auto
+      moreover
+      { assume "t' < t"
+        hence 0: " worldline t \<sigma> \<theta> \<tau>' s' t' =  signal_of2 False \<theta> s' t'"
+          unfolding worldline_def by auto
+        have "t' < t + dly"
+          using `t' < t` by auto
+        hence "w[sig, t + dly := beval_world w t exp] s' t' = worldline t \<sigma> \<theta> \<tau> s' t'"
+          unfolding `w = worldline t \<sigma> \<theta> \<tau>` worldline_upd_def by auto
+        also have "... = signal_of2 False \<theta> s' t'"
+          using `t' < t` unfolding worldline_def by auto
+        finally have "w[sig, t + dly := beval_world w t exp] s' t' = signal_of2 False \<theta> s' t'"
+          by auto
+        hence "worldline t \<sigma> \<theta> \<tau>' s' t' = w[sig, t + dly := beval_world w t exp] s' t'"
+          using 0 by auto }
+      moreover
+      { assume "t' \<ge> t"
+        hence 0: "worldline t \<sigma> \<theta> \<tau>' s' t' = signal_of2 (\<sigma> s') \<tau>' s' t'"
+          unfolding worldline_def by auto
+        have "t' < t + dly \<or> t' \<ge> t + dly"
+          by auto
+        moreover
+        { assume "t' < t + dly"
+          have "w[sig, t + dly := beval_world w t exp] s' t' = worldline t \<sigma> \<theta> \<tau> s' t'"
+            using `t' < t + dly` unfolding `w = worldline t \<sigma> \<theta> \<tau>` worldline_upd_def by auto
+          also have "... = signal_of2 (\<sigma> s') \<tau> s' t'"
+            using `t' \<ge> t` unfolding worldline_def by auto
+          finally have 1: "w[sig, t + dly := beval_world w t exp] s' t' = signal_of2 (\<sigma> s') \<tau> s' t'"
+            by auto
+
+          have "worldline t \<sigma> \<theta> \<tau>' s' t' = signal_of2 (\<sigma> s') \<tau>' s' t'"
+            using `t' \<ge> t` unfolding worldline_def by auto
+          also have "... = signal_of2 (\<sigma> s') \<tau> s' t'"
+            using signal_of_trans_post2[OF `t' < t + dly`] unfolding \<tau>'_def by metis
+          also have "... = w[sig, t + dly := beval_world w t exp] s' t'"
+            using 1 by auto
+          finally have "worldline t \<sigma> \<theta> \<tau>' s' t' = w[sig, t + dly := beval_world w t exp] s' t'"
+            by auto }
+        moreover
+        { assume "t' \<ge> t + dly"
+          have "s' = sig \<or> s' \<noteq> sig" by auto
+          moreover
+          { assume "s' = sig"
+            hence 2: "w[sig, t + dly := beval_world w t exp] s' t' = beval_world (worldline t \<sigma> \<theta> \<tau>) t exp"
+              using `t' \<ge> t + dly` unfolding `w = worldline t \<sigma> \<theta> \<tau>` worldline_upd_def by auto
+            have "worldline t \<sigma> \<theta> \<tau>' s' t' = signal_of2 (\<sigma> s') \<tau>' s' t'"
+              using `t' \<ge> t` unfolding worldline_def by auto
+            also have "... = beval_world (worldline t \<sigma> \<theta> \<tau>) t exp"
+              using signal_of_trans_post3[OF `t + dly \<le> t'`, of "\<sigma> s'" "sig"] unfolding \<tau>'_def
+              `w = worldline t \<sigma> \<theta> \<tau>` by (simp add: \<open>s' = sig\<close>)
+            finally have "worldline t \<sigma> \<theta> \<tau>' s' t' = w[sig, t + dly := beval_world w t exp] s' t' "
+              using 2 by auto }
+          moreover
+          { assume "s' \<noteq> sig"
+            hence "sig \<noteq> s'" by auto
+            hence "w[sig, t + dly := beval_world w t exp] s' t' = worldline t \<sigma> \<theta> \<tau> s' t'"
+              unfolding `w = worldline t \<sigma> \<theta> \<tau>` worldline_upd_def  by auto
+            also have "... = signal_of2 (\<sigma> s') \<tau> s' t'"
+              using `t' \<ge> t` unfolding worldline_def by auto
+            finally have 3: "w[sig, t + dly := beval_world w t exp] s' t' = signal_of2 (\<sigma> s') \<tau> s' t'"
+              by auto
+            have "worldline t \<sigma> \<theta> \<tau>' s' t' = signal_of2 (\<sigma> s') \<tau>' s' t'"
+              using `t' \<ge> t` unfolding worldline_def by auto
+            also have "... = signal_of2 (\<sigma> s') \<tau> s' t'"
+              unfolding \<tau>'_def using signal_of_trans_post[OF `sig \<noteq> s'`] by metis
+            also have "... = w[sig, t + dly := beval_world w t exp] s' t'"
+              using 3 by auto
+            finally have "worldline t \<sigma> \<theta> \<tau>' s' t' = w[sig, t + dly := beval_world w t exp] s' t' "
+              by auto }
+          ultimately have "worldline t \<sigma> \<theta> \<tau>' s' t' = w[sig, t + dly := beval_world w t exp] s' t' "
+            by auto }
+        ultimately have "worldline t \<sigma> \<theta> \<tau>' s' t' = w[sig, t + dly := beval_world w t exp] s' t' "
+          by auto }
+      ultimately show "worldline t \<sigma> \<theta> \<tau>' s' t' = w[sig, t + dly := beval_world w t exp] s' t'"
+        by auto
+    qed
+    with imp and `P w` have "Q(w[sig, t + dly := beval_world w t exp])"
+      by auto
+    assume "w' = worldline t \<sigma> \<theta> \<tau>'"
+    hence "Q w'"
+      using `Q(w[sig, t + dly := beval_world w t exp])` `worldline t \<sigma> \<theta> \<tau>' = w[sig, t + dly := beval_world w t exp]`
+      by auto }
+  thus " \<Turnstile>\<^sub>t {P} Bassign_trans sig exp dly {Q}"
+    unfolding seq_hoare_valid_def by auto
+qed
+
+lemma Bassign_inert_sound:
+  assumes "0 < dly"
+  shows "\<turnstile>\<^sub>t {P} Bassign_inert sig exp dly {Q} \<Longrightarrow> \<Turnstile>\<^sub>t {P} Bassign_inert sig exp dly {Q}"
+proof -
+  assume "\<turnstile>\<^sub>t {P} Bassign_inert sig exp dly {Q}"
+  hence imp: "\<forall>w. P w \<longrightarrow> Q(w[sig, t + dly, t := beval_world w t exp])"
+    by (auto dest!: Bassign_inertE)
+  { fix \<sigma> :: "'a state"
+    fix \<tau> \<tau>' \<theta> :: "'a transaction"
+    fix w w' :: "'a worldline"
+    fix \<gamma>
+    assume c: "context_invariant t \<sigma> \<gamma> \<theta> \<tau>"
+    assume "w = worldline t \<sigma> \<theta> \<tau>"
+    assume "P w"
+    assume ex: "t, \<sigma>, \<gamma>, \<theta> \<turnstile> <Bassign_inert sig exp dly, \<tau>> \<longrightarrow>\<^sub>s \<tau>'"
+    hence "\<tau>' = inr_post sig (beval t \<sigma> \<gamma> \<theta> exp) (\<sigma> sig) \<tau> t dly"
+      by auto
+    moreover have "beval t \<sigma> \<gamma> \<theta> exp = beval_world w t exp"
+      using `w = worldline t \<sigma> \<theta> \<tau>`  `context_invariant t \<sigma> \<gamma> \<theta> \<tau>`
+      unfolding context_invariant_def by (simp add: beval_beval_world)
+    ultimately have \<tau>'_def: "\<tau>' = inr_post sig (beval_world w t exp) (\<sigma> sig) \<tau> t dly"
+      by auto
+    have "\<And>n. n < t \<Longrightarrow> lookup \<tau> n = 0"
+      using `context_invariant t \<sigma> \<gamma> \<theta> \<tau>` unfolding context_invariant_def by auto
+    hence "\<And>n. n < t \<Longrightarrow> lookup \<tau>' n = 0"
+      unfolding \<tau>'_def using inr_post_preserve_trans_removal by metis
+    have nn: "nonneg_delay (Bassign_inert sig exp dly)"
+      using `0 < dly` by auto
+    have "context_invariant t \<sigma> \<gamma> \<theta> \<tau>'"
+      using b_seq_exec_preserves_context_invariant[OF c ex nn] by auto
+    hence asm: "\<forall>s. s \<in> dom (get_trans \<tau>' t) \<longrightarrow> \<sigma> s = the (get_trans \<tau>' t s)"
+      unfolding context_invariant_def by auto
+    hence asm': "\<forall>s. s \<in> dom (get_trans \<tau> t) \<longrightarrow> \<sigma> s = the (get_trans \<tau> t s)"
+      using `context_invariant t \<sigma> \<gamma> \<theta> \<tau>` unfolding context_invariant_def by auto
+    have "worldline t \<sigma> \<theta> \<tau>' = w[sig, t + dly, t := beval_world w t exp]"
+    proof (rule ext, rule ext)
+      fix s' t'
+      have "s' \<noteq> sig \<or> t' < t \<or> s' = sig \<and> t \<le> t'"
+        by auto
+      moreover
+      { assume "s' \<noteq> sig \<or> t' < t"
+        moreover
+        { assume "t' < t"
+          hence 0: " worldline t \<sigma> \<theta> \<tau>' s' t' =  signal_of2 False \<theta> s' t'"
+            unfolding worldline_def by auto
+          have "t' < t + dly"
+            using `t' < t` by auto
+          hence "w[sig, t + dly, t := beval_world w t exp] s' t' = worldline t \<sigma> \<theta> \<tau> s' t'"
+            unfolding `w = worldline t \<sigma> \<theta> \<tau>` worldline_inert_upd_def  by (simp add: \<open>t' < t\<close>)
+          also have "... = signal_of2 False \<theta> s' t'"
+            using `t' < t` unfolding worldline_def by auto
+          finally have "w[sig, t + dly, t := beval_world w t exp] s' t' = signal_of2 False \<theta> s' t'"
+            by auto
+          hence "worldline t \<sigma> \<theta> \<tau>' s' t' = w[sig, t + dly, t := beval_world w t exp] s' t'"
+            using 0 by auto }
+        moreover
+        { assume "s' \<noteq> sig"
+          hence "w[sig, t + dly, t := beval_world w t exp] s' t' = worldline t \<sigma> \<theta> \<tau> s' t'"
+            unfolding worldline_inert_upd_def `w = worldline t \<sigma> \<theta> \<tau>` by auto
+          also have "... = worldline t \<sigma> \<theta> \<tau>' s' t'"
+          proof -
+            have "\<And>n. lookup (to_transaction2 \<tau> s') n = lookup (to_transaction2 \<tau>' s') n"
+              using `s' \<noteq> sig` unfolding \<tau>'_def inr_post_def apply transfer' unfolding to_trans_raw2_def
+              trans_post_raw_def  by (simp add: purge_raw_does_not_affect_other_sig)
+            hence "signal_of2 (\<sigma> s') \<tau> s' t' = signal_of2 (\<sigma> s') \<tau>'  s' t'"
+              using signal_of2_lookup_sig_same  by metis
+            thus ?thesis
+              unfolding worldline_def by auto
+          qed
+          finally have "worldline t \<sigma> \<theta> \<tau>' s' t' = w[sig, t + dly, t := beval_world w t exp] s' t'"
+            by auto }
+        ultimately have "worldline t \<sigma> \<theta> \<tau>' s' t' = w[sig, t + dly, t := beval_world w t exp] s' t'"
+          by auto }
+      moreover
+      { assume "s' = sig \<and> t \<le> t'"
+        hence "t + dly \<le> t' \<or> t' < t + dly" and "s' = sig" and "t \<le> t'"
+          by auto
+        moreover
+        { assume "t + dly \<le> t'"
+          hence 2: "w[sig, t + dly, t := beval_world w t exp] s' t' = beval_world (worldline t \<sigma> \<theta> \<tau>) t exp"
+              using `s' = sig` unfolding `w = worldline t \<sigma> \<theta> \<tau>` worldline_inert_upd_def by auto
+          have "worldline t \<sigma> \<theta> \<tau>' s' t' = signal_of2 (\<sigma> s') \<tau>' s' t'"
+            using `t' \<ge> t` unfolding worldline_def by auto
+          also have "... = beval_world (worldline t \<sigma> \<theta> \<tau>) t exp"
+            using signal_of_inr_post[OF `t + dly \<le> t'`, of "\<sigma> s'" "sig"] unfolding \<tau>'_def
+            `w = worldline t \<sigma> \<theta> \<tau>` by (simp add: \<open>s' = sig \<and> t \<le> t'\<close>)
+          finally have "worldline t \<sigma> \<theta> \<tau>' s' t' = w[sig, t + dly, t := beval_world w t exp] s' t' "
+            using 2 by auto }
+        moreover
+        { assume "t' < t + dly"
+          hence "w[sig, t + dly, t := beval_world w t exp] s' t' = w sig t"
+            unfolding worldline_inert_upd_def using `s' = sig`  using \<open>s' = sig \<and> t \<le> t'\<close> by auto
+          also have "... = signal_of2 (\<sigma> sig) \<tau> sig t"
+            unfolding `w = worldline t \<sigma> \<theta> \<tau>` worldline_def by auto
+          also have "... = \<sigma> sig"
+          proof (cases "lookup \<tau> t sig = None")
+            case True
+            have "\<And>k. k \<in>dom (lookup (to_transaction2 \<tau> sig)) \<Longrightarrow> t < k"
+            proof (rule ccontr)
+              fix k
+              assume in_dom: "k \<in>dom (lookup (to_transaction2 \<tau> sig))"
+              assume "\<not> t < k" hence "k \<le> t" by auto
+              hence "lookup \<tau> k sig = None"
+                using `\<And>n. n < t \<Longrightarrow> lookup \<tau> n = 0` True  by (metis dual_order.antisym leI zero_map)
+              hence "k \<notin> dom (lookup (to_transaction2 \<tau> sig))"
+                apply transfer' unfolding to_trans_raw2_def by auto
+              with in_dom show "False" by auto
+            qed
+            hence "inf_time (to_transaction2 \<tau>) sig t = None"
+              by (simp add: inf_time_noneI)
+            then show ?thesis
+              unfolding to_signal2_def comp_def by auto
+          next
+            case False
+            hence "lookup \<tau> t sig = Some (\<sigma> sig)"
+              using asm'  by (simp add: domIff)
+            with lookup_some_signal_of2' show ?thesis
+              by fastforce
+          qed
+          finally have l: "w[sig, t + dly, t := beval_world w t exp] s' t' = \<sigma> sig"
+            by auto
+
+          have "worldline t \<sigma> \<theta> \<tau>' s' t' = signal_of2 (\<sigma> s') \<tau>' s' t'"
+            unfolding worldline_def using `s' = sig \<and> t \<le> t'` by auto
+          also have "... = \<sigma> s'"
+            using signal_of_inr_post2[OF `t \<le> t'` `t' < t + dly` `\<And>n. n < t \<Longrightarrow> lookup \<tau> n = 0` asm', of "s'"]
+            unfolding \<tau>'_def using `s' = sig` by auto
+          finally have "worldline t \<sigma> \<theta> \<tau>' s' t' = \<sigma> s'"
+            by auto
+          with l have "worldline t \<sigma> \<theta> \<tau>' s' t' = w[sig, t + dly, t := beval_world w t exp] s' t' "
+            using `s' = sig` by auto }
+        ultimately have "worldline t \<sigma> \<theta> \<tau>' s' t' = w[sig, t + dly, t := beval_world w t exp] s' t' "
+          by auto }
+      ultimately show "worldline t \<sigma> \<theta> \<tau>' s' t' = w[sig, t + dly, t := beval_world w t exp] s' t' "
+        by auto
+    qed
+    with imp and `P w` have "Q(w[sig, t + dly, t := beval_world w t exp])"
+      by auto
+    assume "w' = worldline t \<sigma> \<theta> \<tau>'"
+    hence "Q w'"
+      using `Q(w[sig, t + dly, t := beval_world w t exp])` `worldline t \<sigma> \<theta> \<tau>' = w[sig, t + dly, t:= beval_world w t exp]`
+      by auto }
+  thus " \<Turnstile>\<^sub>t {P} Bassign_inert sig exp dly {Q}"
+    unfolding seq_hoare_valid_def by auto
+qed
+
+lemma soundness:
+  assumes "\<turnstile>\<^sub>t {P} s {R}"
+  assumes "nonneg_delay s"
+  shows "\<Turnstile>\<^sub>t {P} s {R}"
+  using assms
+proof (induction rule:seq_hoare.induct)
+  case (AssignI t P sig dly exp)
+  hence "0 < dly" by auto
+  then show ?case
+    using Bassign_inert_sound[OF `0 < dly`]  using seq_hoare.AssignI by fastforce
+next
+  case (Conseq P' P t s Q Q')
+  then show ?case  by (auto simp add: seq_hoare_valid_def)
+qed (auto simp add: Bnull_sound Bassign_trans_sound Bcomp_hoare_valid Bguarded_hoare_valid)
+
+end
